Add examples for oneshot ghost variable and nested invariant proofs

Freesia_model/client/example_oneshot_ghost_variable.v
@@ -1,39 +1,44 @@
-From iris.algebra Require Import frac agree csum.
 From iris.proofmode Require Import tactics.
-From iris.program_logic Require Export weakestpre.
 From iris.heap_lang Require Export lang.
 From iris.heap_lang Require Import assert proofmode notation adequacy.
 From iris.heap_lang.lib Require Import par.
-From iris.prelude Require Import options.
 
-From lib Require Import basic_types.
 From lib Require Import oneshot.
 From core.kernel Require Import spinlock.
 
 Context `{!heapGS Σ, !oneshotG Σ, !spawnG Σ}.
 
+(** Concurrent increment with spinlock using oneshot ghost variables *)
 Definition incr_inner : val := λ: "ℓ" "flag",
+  (* Attempt to acquire flag and increment ℓ if successful *)
   if: !"flag" = #false then
-    "flag" <- #true;;
-    FAA "ℓ" #1;;
+    "flag" <- #true;;          (* Set flag to mark critical section *)
+    FAA "ℓ" #1;;              (* Atomic increment *)
     #()
   else
-    #().
+    #().                      (* Already locked, no-op *)
 
+(** Main increment operation with spinlock protection *)
 Definition incr : val := λ: "lk" "ℓ" "flag",
-  cpu_spin_lock "lk";;
-  incr_inner "ℓ" "flag";;
-  cpu_spin_unlock "lk".
+  cpu_spin_lock "lk";;         (* Acquire spinlock *)
+  incr_inner "ℓ" "flag";;      (* Perform actual increment *)
+  cpu_spin_unlock "lk".        (* Release spinlock *)
 
+(** Parallel execution of two increment operations *)
 Definition parallel_incr : val := λ: "lk" "ℓ" "flag",
+  (* Fork two threads *)
   (incr "lk" "ℓ" "flag") ||| (incr "lk" "ℓ" "flag");;
-  ! "ℓ".
+  ! "ℓ".                      (* Return final value *)
 
+(** Invariant combining physical state and ghost state:
+    - flag: physical variable status
+    - ℓ: shared counter
+    - γ: oneshot ghost variable tracking completion *)
 Definition incr_inv (ℓ : loc) (flag : loc) (γ : gname) (n : Z) : iProp Σ :=
-    (flag ↦ #false ∗ ℓ ↦ #n ∗ (Pending γ (1/2)%Qp)
-  ∨ flag ↦ #true ∗ ℓ ↦ #(n+1) ∗ (Shot γ #(n+1)))%I.
+    (flag ↦ #false ∗ ℓ ↦ #n ∗ (Pending γ (1/2)%Qp)     (* pending state *)
+  ∨ flag ↦ #true ∗ ℓ ↦ #(n+1) ∗ (Shot γ #(n+1)))%I.     (* shot state *)
 
-
+(** Verification of successful incr execution *)
 Lemma incr_succ_spec (lk : loc) (ℓ : loc) (flag : loc) (n : Z) (γ : gname):
   {{{ flag ↦ #false ∗
       (Pending γ (1/2)%Qp) ∗
@@ -43,26 +48,37 @@ Lemma incr_succ_spec (lk : loc) (ℓ : loc) (flag : loc) (n : Z) (γ : gname):
 Proof.
   iIntros "%Φ [Hflag [Hγ1 #Hsp]] HΦ /=".
   wp_lam. wp_let. wp_let.
+
+  (* 1. Acquire spinlock and open invariant *)
   wp_bind (cpu_spin_lock _).
   wp_apply (cpu_spin_lock_spec with "Hsp").
   iIntros "[Hinv_sp Hinv_incr]".
   wp_seq. wp_lam. wp_let.
+
+  (* 2. Case analysis on current state *)
   wp_bind (! _)%E.
   iDestruct "Hinv_incr" as "[[_ [Hl Hγ2]]|[_ [Hl Hγ2]]]".
-  - (* Case 1: flag ↦ #false ∗ ℓ ↦ #n *)
+  - (* Case 1: pending state *)
     wp_load. wp_pures. wp_store.
+
+    (* 3. Split and shoot oneshot *)
     iDestruct (pending_split with "[$Hγ1 $Hγ2]") as "Hγ".
     iMod (pending_shoot _ #(n+1) with "Hγ") as "Hγ".
     iAssert ((Shot γ #(n+1)) ∗ (Shot γ #(n+1)))%I with "[Hγ]" as "[Hγ1 Hγ2]".
     { by iApply shot_idemp. }
+
+    (* 4. Perform atomic increment *)
     wp_faa. wp_seq. wp_seq.
+
+    (* 5. Release lock with updated state *)
     wp_apply (cpu_spin_unlock_spec with "[Hinv_sp Hflag Hl Hγ1]").
     * iFrame. iRight. iFrame.
     * iIntros "_". iApply "HΦ". iApply "Hγ2".
-  - (* Case 2: flag ↦ #true ∗ ℓ ↦ #(n+1) *)
+  - (* Case 2: shot state (already completed)  *)
     by iCombine "Hγ1 Hγ2" gives %?.
 Qed.
 
+(** Verification of failed incr execution *)
 Lemma incr_failed_spec (lk : loc) (ℓ : loc) (flag : loc) (n : Z) (γ : gname):
   {{{ flag ↦ #true ∗
       is_spinlock #lk (incr_inv ℓ flag γ n) }}}
@@ -71,29 +87,37 @@ Lemma incr_failed_spec (lk : loc) (ℓ : loc) (flag : loc) (n : Z) (γ : gname):
 Proof.
   iIntros "%Φ [Hflag #Hsp] HΦ /=".
   wp_lam. wp_let. wp_let.
+
+  (* 1. Acquire spinlock and open invariant *)
   wp_bind (cpu_spin_lock _).
   wp_apply (cpu_spin_lock_spec with "Hsp").
   iIntros "[Hinv_sp Hinv_incr]".
   wp_seq. wp_lam. wp_let.
+
+  (* 2. Case analysis on current state *)
   wp_bind (! _)%E.
   iDestruct "Hinv_incr" as "[[H [Hl Hγ2]]|[_ [Hl Hγ2]]]".
-  - (* Case 1: flag ↦ #false ∗ ℓ ↦ #n *)
-    iAssert (False)%I with "[H Hflag]" as %[].
+  - (* Case 1: pending state *)
+    iAssert (False)%I with "[H Hflag]" as %[].    (* exfalso situation *)
     { iApply (pointsto_exclusive flag). iFrame. }
-  - (* Case 2: flag ↦ #true ∗ ℓ ↦ #(n+1) *)
+  - (* Case 2: shot state *)
     wp_load. wp_pures.
+
+    (* 3. shot idempotent *)
     iAssert ((Shot γ #(n+1)) ∗ (Shot γ #(n+1)))%I with "[Hγ2]" as "[Hγ1 Hγ2]".
     { by iApply shot_idemp. }
+
+    (* 4. Release lock with Nop *)
     wp_apply (cpu_spin_unlock_spec with "[Hinv_sp Hflag Hl Hγ1]").
     * iFrame. iRight. iFrame.
     * iIntros "_". iApply "HΦ". iApply "Hγ2".
 Qed.
 
-
+(** Verification of successful inner incr operation *)
 Lemma incr_inner_succ_spec (ℓ : loc) (flag : loc) (n : Z) (γ : gname):
-  {{{ flag ↦ #false ∗
-      ℓ ↦ #n ∗
-      (Pending γ 1%Qp) }}}
+  {{{ flag ↦ #false ∗             (* Physical flag in unlocked state *)
+      ℓ ↦ #n ∗                    (* Shared counter value *)
+      (Pending γ 1%Qp) }}}        (* Full pending ghost state *)
     incr_inner #ℓ #flag
   {{{ RET #(); (Shot γ #(n+1)) ∗ incr_inv ℓ flag γ n }}}.
 Proof.
@@ -101,139 +125,184 @@ Proof.
   wp_lam. wp_let.
   wp_bind (! _)%E.
   wp_load. wp_pures. wp_store.
+
+  (* Ghost state transition *)
   iMod (pending_shoot _ #(n+1) with "Hγ") as "Hγ".
+  (* Idempotency of shot *)
   iAssert ((Shot γ #(n+1)) ∗ (Shot γ #(n+1)))%I with "[Hγ]" as "[Hγ1 Hγ2]".
     { by iApply shot_idemp. }
+
   wp_faa. wp_seq.
   iModIntro. iApply "HΦ".
+  
+  (* construct invariant *)
   iFrame. iRight. iFrame.
 Qed.
 
+(** Verification of failed inner incr operation *)
 Lemma incr_inner_failed_spec (ℓ : loc) (flag : loc) (n : Z) (γ : gname):
-  {{{ flag ↦ #true ∗
-      ℓ ↦ #(n+1) ∗
-      (Shot γ #(n+1)) }}}
+  {{{ flag ↦ #true ∗            (* Physical flag already locked *)
+      ℓ ↦ #(n+1) ∗              (* Pre-incremented counter *)
+      (Shot γ #(n+1)) }}}       (* Existing shot ghost state *)
     incr_inner #ℓ #flag
   {{{ RET #(); (Shot γ #(n+1)) ∗ incr_inv ℓ flag γ n }}}.
 Proof.
   iIntros "%Φ [Hflag [Hl Hγ]] HΦ /=".
+
+  (* Leverage shot idempotency *)
   iAssert ((Shot γ #(n+1)) ∗ (Shot γ #(n+1)))%I with "[Hγ]" as "[Hγ1 Hγ2]".
     { by iApply shot_idemp. }
+
   wp_lam. wp_let.
   wp_bind (! _)%E.
   wp_load. wp_pures.
   iModIntro. iApply "HΦ".
+
+  (* construct invariant *)
   iFrame. iRight. iFrame.
 Qed.
 
-
+(** Structural decomposition lemma for pending state *)
 Lemma incr_inv_pending (ℓ : loc) (flag : loc) (n : Z) (γ : gname):
   incr_inv ℓ flag γ n ∗ (Pending γ (1/2)%Qp) -∗
   flag ↦ #false ∗ ℓ ↦ #n ∗ (Pending γ (1/2)%Qp).
 Proof.
   iIntros "[Hinv_incr Hγ1]".
+  (* Case analysis *)
   iDestruct "Hinv_incr" as "[[Hflag [Hl Hγ2]]|[Hflag [Hl Hγ2]]]".
-  - iFrame.
-  - by iCombine "Hγ1 Hγ2" gives %?.
+  - iFrame.                           (* Left case: pending state *)
+  - by iCombine "Hγ1 Hγ2" gives %?.   (* Right case: contradiction *)
 Qed.
 
+(** Structural decomposition lemma for shot state *)
 Lemma incr_inv_shot (ℓ : loc) (flag : loc) (n : Z) (γ : gname):
   incr_inv ℓ flag γ n ∗ (Shot γ #(n+1)) -∗
   flag ↦ #true ∗ ℓ ↦ #(n+1) ∗ (Shot γ #(n+1)).
 Proof.
   iIntros "[Hinv_incr Hγ1]".
+  (* Case analysis *)
   iDestruct "Hinv_incr" as "[[Hflag [Hl Hγ2]]|[Hflag [Hl Hγ2]]]".
-  - by iCombine "Hγ1 Hγ2" gives %?.
-  - iFrame.
+  - by iCombine "Hγ1 Hγ2" gives %?.   (* Left case: contradiction *)
+  - iFrame.                           (* Right case: shot state *)
 Qed.
 
+(** Full initialization and increment specification *)
 Lemma incr_spec1 (lk : loc) (ℓ : loc) (flag : loc) (n : Z) (γ : gname):
-  {{{ flag ↦ #false ∗ ℓ ↦ #n ∗ lk ↦ #false ∗
-      (Pending γ 1%Qp) }}}
+  {{{ flag ↦ #false ∗                    (* Physical flag in unlocked state *)
+      ℓ ↦ #n ∗                           (* Shared counter initial value *)
+      lk ↦ #false ∗                      (* Spinlock in unlocked state *)
+      (Pending γ 1%Qp) }}}               (* Full pending ghost resource *)
     incr #lk #ℓ #flag
-  {{{ RET #(); (Shot γ #(n+1)) }}}.
+  {{{ RET #(); (Shot γ #(n+1)) }}}.      (* Postcondition: shot state *)
 Proof.
   iIntros "%Φ [Hflag [Hl [Hlk Hγ]]] HΦ /=".
   wp_lam.
   wp_let. wp_let.
-  (* iMod (own_alloc (Pending 1%Qp)) as (γ) "Hγ"; first done. *)
+
+  (* 1. Split pending ghost resource *)
   iDestruct (pending_split with "Hγ") as "[Hγ1 Hγ2]".
-  (* iMod (inv_alloc N _ (incr_inv ℓ flag γ n) with "[Hflag Hl Hγ2]") as "#Hinv_incr".
-  { iLeft. by iFrame. } *)
+
+  (* 2. Establish increment invariant *)
   iAssert (incr_inv ℓ flag γ n)%I with "[Hflag Hl Hγ2]" as "Hinv_incr".
-  { iLeft. by iFrame. }
+  { iLeft. by iFrame. }     (* Left disjunct: pending state *)
+
+  (* 3. Create spinlock invariant *)
   iMod (inv_alloc basic_types.lockN _ (spinlock_inv lk ((incr_inv ℓ flag γ n))) with "[Hlk Hinv_incr]") as "#Hinv_sp".
-  { iNext. iExists false. iFrame. }
-  (* iMod (inv_alloc N _ (is_spinlock #lk (inv N (incr_inv ℓ flag γ n))) with "[Hinv]") as "#HN".
-  { iNext. iExists lk. iSplit; first eauto. iExact "Hinv". } *)
+  { iNext. iExists false. iFrame. }       (* Initial lock state: unlocked *)
+
+  (* 4. Cast to spinlock interface *)
   iAssert (is_spinlock #lk ((incr_inv ℓ flag γ n))) with "[Hinv_sp]" as "#Hinv".
   { iExists lk. iSplit; first eauto. iExact "Hinv_sp". }
+
+  (* 5. Main lock-protected increment *)
   wp_bind (cpu_spin_lock _).
   wp_apply (cpu_spin_lock_spec with "Hinv").
   iIntros "[Hinv1 Hinv_incr]".
   wp_seq.
   wp_bind (incr_inner _ _).
+
+  (* 6. Case analysis on shared state *)
   iDestruct "Hinv_incr" as "[[Hflag [Hl Hγ2]]|[Hflag [Hl Hγ2]]]".
-  - iDestruct (pending_split with "[$Hγ1 $Hγ2]") as "Hγ".
-    (* iApply incr_inner_succ_spec. *)
+  - (* Case: pending state *)
+    iDestruct (pending_split with "[$Hγ1 $Hγ2]") as "Hγ".
     wp_apply (incr_inner_succ_spec ℓ flag n γ with "[Hflag Hl Hγ]").
     { iFrame. }
     iIntros "[Hγ Hinv_incr]".
     wp_seq.
+    (* 7. Release spinlock *)
     wp_apply (cpu_spin_unlock_spec with "[Hinv1 Hinv_incr]").
-    + iFrame. iApply "Hinv_incr".
+    + iFrame. iApply "Hinv_incr".     (* Reconstruct lock invariant *)
     + iIntros "_". iApply "HΦ". iApply "Hγ".
-  - by iCombine "Hγ1 Hγ2" gives %?.
+  - (* Case: shot state *)
+    by iCombine "Hγ1 Hγ2" gives %?.   (* pending + shot contradiction *)
 Qed.
 
+(** General increment specification with existing lock *)
 Lemma incr_spec (lk : loc) (ℓ : loc) (flag : loc) (n : Z) (γ : gname):
-  {{{ is_spinlock #lk (incr_inv ℓ flag γ n) ∗
-      (Pending γ (1/2)%Qp) }}}
+  {{{ is_spinlock #lk (incr_inv ℓ flag γ n) ∗  (* Existing lock invariant *)
+      (Pending γ (1/2)%Qp) }}}                 (* Half pending ghost resource *)
     incr #lk #ℓ #flag
   {{{ RET #(); (Shot γ #(n+1)) }}}.
 Proof.
   iIntros "%Φ [#Hinv Hγ1] HΦ /=".
-  wp_lam.
-  wp_let. wp_let.
+  wp_lam. wp_let. wp_let.
+
+  (* 1. Acquire spinlock *)
   wp_bind (cpu_spin_lock _).
   wp_apply (cpu_spin_lock_spec with "Hinv").
   iIntros "[Hinv1 Hinv_incr]".
   wp_seq.
   wp_bind (incr_inner _ _).
+
+  (* 2. State decomposition *)
   iDestruct "Hinv_incr" as "[[Hflag [Hl Hγ2]]|[Hflag [Hl Hγ2]]]".
-  - iDestruct (pending_split with "[$Hγ1 $Hγ2]") as "Hγ".
-    (* iApply incr_inner_succ_spec. *)
+  - (* Case: pending state *)
+    iDestruct (pending_split with "[$Hγ1 $Hγ2]") as "Hγ".
     wp_apply (incr_inner_succ_spec ℓ flag n γ with "[Hflag Hl Hγ]").
     { iFrame. }
     iIntros "[Hγ Hinv_incr]".
     wp_seq.
+    (* 3. Release spinlock *)
     wp_apply (cpu_spin_unlock_spec with "[Hinv1 Hinv_incr]").
-    + iFrame. iApply "Hinv_incr".
+    + iFrame. iApply "Hinv_incr".     (* Reconstruct lock invariant *)
     + iIntros "_". iApply "HΦ". iApply "Hγ".
-  - by iCombine "Hγ1 Hγ2" gives %?.
+  - (* Case: shot state *)
+    by iCombine "Hγ1 Hγ2" gives %?.       (* Resource contradiction *)
 Qed.
 
+(** Parallel increment verification *)
 Lemma parallel_incr_spec (lk : loc) (ℓ : loc) (flag : loc) (n : Z) (γ : gname):
-  {{{ is_spinlock #lk (incr_inv ℓ flag γ n) ∗
-      incr_inv ℓ flag γ n ∗
-      (Pending γ 1%Qp) }}}
+  {{{ is_spinlock #lk (incr_inv ℓ flag γ n) ∗  (* Lock invariant *)
+      incr_inv ℓ flag γ n ∗                    (* Current shared state *)
+      (Pending γ 1%Qp) }}}                     (* Full pending ghost resource *)
     parallel_incr #lk #ℓ #flag
   {{{ RET #(n+1); True }}}.
 Proof.
   iIntros "%Φ [#Hinv [Hinv_incr Hγ]] HΦ /=".
+
+  (* 1. Split ghost resource for parallel threads *)
   iDestruct (pending_split with "Hγ") as "[Hγ1 Hγ2]".
   wp_lam. wp_let. wp_let.
-  wp_smart_apply (wp_par (λ _ , (Shot γ #(n+1))) (λ _ , (Shot γ #(n+1))) with "[Hγ1] [Hγ2]").
-  - wp_apply (incr_spec with "[Hinv Hγ1]").
+
+  (* 2. Parallel execution *)
+  wp_smart_apply (wp_par 
+    (λ _, Shot γ #(n+1))                 (* Left thread postcondition *)
+    (λ _, Shot γ #(n+1))                 (* Right thread postcondition *)
+    with "[Hγ1] [Hγ2]").
+  - (* Left thread *)
+    wp_apply (incr_spec with "[Hinv Hγ1]").
     + iFrame. iApply "Hinv".
     + iIntros "Hγ". iApply "Hγ".
-  - wp_apply (incr_spec with "[Hinv Hγ2]").
+  - (* Right thread *)
+    wp_apply (incr_spec with "[Hinv Hγ2]").
     + iFrame. iApply "Hinv".
     + iIntros "Hγ". iApply "Hγ".
-  - iIntros (v1 v2) "[Hγ1 Hγ2]".
+  - (* Post-parallel join *)
+    iIntros (v1 v2) "[Hγ1 Hγ2]".
     iModIntro. wp_seq.
+
+    (* 3. Verify final state *)
     iAssert (flag ↦ #true ∗ ℓ ↦ #(n+1) ∗ (Shot γ #(n+1)))%I with "[Hinv_incr Hγ1]" as "[Hflag [Hl Hγ3]]".
     { iApply incr_inv_shot. iFrame. }
     wp_load. iModIntro. iApply "HΦ". done.
 Qed.
-
