Freesia_model/client/example_nested_invariant.v
@@ -1,0 +1,63 @@
+From iris.proofmode Require Import tactics.
+From iris.heap_lang Require Export lang.
+From iris.heap_lang Require Import assert proofmode notation adequacy.
+From iris.base_logic Require Import invariants ghost_var.
+
+Context `{!heapGS Σ}.
+
+(* Declare namespaces *)
+Definition outer_ns := nroot .@ "outer".
+Definition inner_ns := nroot .@ "inner".
+
+(* Inner invariant: enforces that integer n is even *)
+Definition inner_inv (n : Z) : iProp Σ :=
+  ⌜Zeven n⌝.
+
+(* Outer invariant: maintains x ↦ n and nests the inner invariant 
+   Note: inner_ns should be declared as a distinct namespace *)
+Definition outer_inv (x : loc) : iProp Σ :=
+  ∃ n:Z, x ↦ #n ∗ inv inner_ns (inner_inv n).
+
+(* Global specification: establishes outer invariant as persistent assertion *)
+Definition is_even (x : loc) : iProp Σ :=
+  inv outer_ns (outer_inv x).
+
+Lemma even_spec (x : loc) :
+  {{{ is_even x }}}
+    #x <- !#x + #2
+  {{{ RET #(); True }}}.
+Proof.
+  iIntros (Φ) "#Hinv_outer Hpost".
+  wp_bind (! _)%E.
+
+  (* Step 1: Open outer invariant to access x's value *)
+  iInv outer_ns as (n) "[Hx #Hinv_inner]" "Hclose".
+  wp_load.  (* Load current value of x *)
+
+  (* Step 2: Verify inner invariant (n must be even) *)
+  iInv "Hinv_inner" as "> %Heven".  (* > indicates later modality *)
+  iModIntro. iSplitR.
+  { iPureIntro. auto. }  (* Re-establish inner invariant unchanged *)
+
+  (* Step 3: Reconstruct outer invariant with original value *)
+  iMod ("Hclose" with "[Hx Hinv_inner]") as "_".
+  { iNext. iFrame. eauto. }  (* Frame unchanged resources *)
+  iModIntro.
+
+  (* Step 4: Prepare new inner invariant for n+2 *)
+  iMod (inv_alloc inner_ns _ (inner_inv (n+2)) 
+    with "[Hinv_inner]") as "#Hinv_inner2".
+  { iNext. iPureIntro. by apply Zeven_plus_Zeven. }  (* n+2 preserves evenness *)
+
+  (* Step 5: Atomic update of x's value *)
+  wp_pure credit:"Hcred".  (* Got a credit *)
+  iInv outer_ns as (n') "[Hx _]" "Hclose".
+  iMod (lc_fupd_elim_later with "Hcred Hx") as "Hx".  (* Eliminate later modality *)
+  wp_store.  (* Store n+2 to x *)
+
+  (* Step 6: Re-establish outer invariant with updated value *)
+  iMod ("Hclose" with "[Hx Hinv_inner]") as "_".
+  { iNext. iExists (n+2)%Z. iFrame. eauto. }  (* Update outer invariant *)
+
+  iModIntro. iApply "Hpost". done.
+Qed.
